busy_beaver/tape.dfy
@@ -1,0 +1,41 @@
+// Generic Tape interface with all necessary post-conditions listed.
+abstract module TapeInterface {
+  type Symbol
+  type Tape
+
+  function Blank(init_symbol : Symbol) : Tape
+    ensures forall pos :: Read(Blank(init_symbol), pos) == init_symbol
+
+  function Read(tape : Tape, pos : int) : Symbol
+
+  function Write(tape : Tape, pos : int, val : Symbol) : Tape
+    ensures Read(Write(tape, pos, val), pos) == val
+    ensures forall p2 :: p2 != pos ==>
+      Read(Write(tape, pos, val), p2) == Read(tape, p2)
+}
+
+// Stack-allocated, non-mutable Tape representation convenient for
+// specification
+module Tape refines TapeInterface {
+  // Generic Symbol type.
+  type Symbol
+
+  datatype Tape = Tape(
+    data : map<int, Symbol>,
+    init_symbol : Symbol
+  )
+
+  function Blank(init_symbol : Symbol) : Tape {
+    Tape(data := map[], init_symbol := init_symbol)
+  }
+
+  function Read(tape : Tape, pos : int) : Symbol {
+    if pos in tape.data then tape.data[pos] else tape.init_symbol
+  }
+
+  // Return a new Tape with update written.
+  function Write(tape : Tape, pos : int, val : Symbol) : Tape {
+    Tape(data := tape.data[pos := val],
+         init_symbol := tape.init_symbol)
+  }
+}
